src/PlutusIR/Semantics/Dynamic/Substitution/Class.v
@@ -1,0 +1,14 @@
+Require Import Coq.Strings.String.
+
+(* Applying substitution of type A on B *)
+Class Subst (A B : Type) := {
+  s : A -> B -> B
+}.
+
+(* Dropping variables from substitutions *)
+Class Drop (A B : Type) := {
+  d : A -> list (string * B) -> list (string * B)
+}.
+
+Notation "γ ⊙ t" := (s γ t) (at level 55, right associativity).
+Notation "γ \\ b" := (d b γ) (at level 50, left associativity).
