src/PlutusIR/Semantics/SemanticEquivalence/LetCons.v
@@ -1,0 +1,105 @@
+From Coq Require Import
+  List
+  Strings.String
+  Lia
+  Program.Equality
+.
+
+From PlutusCert Require Import Semantics.Dynamic.
+From PlutusCert Require Import Semantics.Static.
+From PlutusCert Require Import BaseKindedness.
+From PlutusCert Require Import SemanticEquivalence.LogicalRelation.
+From PlutusCert Require Import SemanticEquivalence.CompatibilityLemmas.
+From PlutusCert Require Import SemanticEquivalence.Auto.
+From PlutusCert Require Import SemanticEquivalence.FundamentalProperty.
+From PlutusCert Require Import Substitution.
+From PlutusCert Require Import Util.Tactics.
+
+From PlutusCert Require Import Multisubstitution.Congruence.
+From PlutusCert Require Import Util.List.
+
+
+From PlutusCert Require Import DeadCode.DSP.Lemmas.
+From PlutusCert Require Import DeadCode.DSP.BoundVars.
+From PlutusCert Require Import Substitution.Free.
+From PlutusCert Require Import SubstitutionPreservesTyping.
+
+Import Utf8_core.
+
+Import ListNotations.
+
+Notation close γ ρ t := (msubst γ (msubstA ρ t)).
+
+(* New LR *)
+Notation "Δ ',,' Γ '|-' e1 ≤ e2 ':' T" := (approx Δ Γ e1 e2 T)
+  ( at level 101
+  , e1 at level 0
+  , e2 at level 0
+  , T at level 0
+  , no associativity).
+
+
+Definition msubstA_LetNonRec (ρ : list (string * ty)) bs e :
+  ρ ⊙ Let NonRec bs e =
+  Let NonRec (ρ ⊙ bs) (ρ - bs ⊙ e).
+Admitted.
+
+Definition msubst_LetNonRec (γ : list (string * term)) bs e :
+  γ ⊙ Let NonRec bs e =
+  Let NonRec (γ ⊙ bs) (γ - bs ⊙ e).
+Admitted.
+
+Definition msubstA_BindingsNonRec_cons
+     : ∀ (ss : list (string * ty)) (b : binding) (bs : list binding),
+         ss ⊙ (b :: bs) =
+         ss ⊙ b :: ss - b ⊙ bs.
+Admitted.
+
+
+Axiom msubst_bnr_cons
+     : ∀ (ss : list (string * term)) (b : binding) (bs : list binding),
+         ss ⊙ (b :: bs) =
+         ss ⊙ b :: ss - b ⊙ bs
+.
+
+Lemma elim_TermBind_NonRec__approximate Δ Γ t Tn b bs:
+  Δ ,, Γ |-+ (Let NonRec (b :: bs) t) : Tn ->
+  Δ ,, Γ |- (Let NonRec (b :: bs) t) ≤ (Let NonRec [b] (Let NonRec bs t)) : Tn.
+Proof.
+  intros H_typing.
+  unfold approx.
+  split; try assumption.
+  split.
+  - admit. (* TODO: typing rules *)
+  - (* C *)
+    intros k ρ γ γ' H_D H_G.
+    autorewrite with R.
+    intros j H_j_k r H_eval_r.
+
+    rewrite msubstA_LetNonRec, msubst_LetNonRec, msubstA_BindingsNonRec_cons,  msubst_bnr_cons
+        in H_eval_r.
+    remember (msyn1 ρ) as ρ₁.
+    remember (msyn2 ρ) as ρ₂.
+      inversion H_eval_r. subst.
+      inversion H3. subst.
+      * (* TermBind *)
+      rewrite <- msubst_LetNonRec in H8.
+      rewrite msubstA_LetNonRec, msubst_LetNonRec, msubstA_BindingsNonRec_cons,  msubst_bnr_cons
+        in H_eval_r.
+      rewrite msubstA_LetNonRec, msubst_LetNonRec, msubstA_BindingsNonRec_cons,  msubst_bnr_cons.
+      constructor.
+      econstructor.
+    eexists. eexists.
+    split.
+    + rewrite msubstA_LetNonRec, msubst_LetNonRec, msubstA_BindingsNonRec_cons,  msubst_bnr_cons
+        in H_eval_r.
+      inversion H_eval_r. subst.
+      inversion H3. subst.
+      * (* TermBind *)
+      rewrite msubstA_LetNonRec, msubst_LetNonRec, msubstA_BindingsNonRec_cons,  msubst_bnr_cons.
+      constructor.
+      econstructor.
+
+    simpl in H_eval_r.
+
+
