src/PlutusIR/Semantics/SemanticEquivalence/LetNil.v
@@ -1,0 +1,127 @@
+From Coq Require Import
+  List
+  Strings.String
+  Lia
+  Program.Equality
+.
+
+From PlutusCert Require Import Semantics.Dynamic.
+From PlutusCert Require Import Semantics.Static.
+From PlutusCert Require Import BaseKindedness.
+From PlutusCert Require Import SemanticEquivalence.LogicalRelation.
+From PlutusCert Require Import SemanticEquivalence.CompatibilityLemmas.
+From PlutusCert Require Import SemanticEquivalence.Auto.
+From PlutusCert Require Import SemanticEquivalence.FundamentalProperty.
+From PlutusCert Require Import Substitution.
+From PlutusCert Require Import Util.Tactics.
+
+From PlutusCert Require Import Multisubstitution.Congruence.
+From PlutusCert Require Import Util.List.
+
+Import PlutusNotations.
+
+From PlutusCert Require Import DeadCode.DSP.Lemmas.
+From PlutusCert Require Import DeadCode.DSP.BoundVars.
+From PlutusCert Require Import Substitution.Free.
+From PlutusCert Require Import SubstitutionPreservesTyping.
+
+Import Utf8_core.
+
+Import ListNotations.
+
+Notation close γ ρ t := (msubst γ (msubstA ρ t)).
+
+
+Lemma has_type__Let_Nil_inv Δ Γ t T :
+  Δ ,, Γ |-+ (Let NonRec [] t) : T ->
+  Δ ,, Γ |-+ t : T.
+Proof.
+    inversion 1. subst.
+    inversion H3. subst.
+    assumption.
+Qed.
+
+Lemma elim_TermBind_NonRec__approximate Δ Γ t Tn :
+  Δ ,, Γ |-+ (Let NonRec [] t) : Tn ->
+  Δ ,, Γ |- (Let NonRec [] t) ≤ t : Tn.
+Proof.
+  intros H_ty.
+  unfold LR_logically_approximate.
+  split; try assumption.
+  split.
+  - (* typing *)
+    inversion H_ty. subst.
+    inversion H2. subst.
+    assumption.
+  -
+    intros k ρ γ γ' H_D H_G.
+    autorewrite with RC.
+    intros j H_j_k r H_eval_r.
+
+      rewrite msubstA_LetNonRec_nil, msubst_LetNonRec_nil  in H_eval_r.
+      inversion H_eval_r. subst.
+      inversion H3. subst.
+      assert (H_refl_t : Δ ,, Γ |- t ≤ t : Tn). {
+        apply LR_reflexivity.
+        inversion H_ty. subst. inversion H4. subst.
+        simpl in H9.
+        assumption.
+      }
+      destruct H_refl_t as [_ [ _ H_C]].
+      specialize (H_C _ ρ γ γ' H_D H_G).
+      autorewrite with RC in H_C.
+      specialize (H_C j1 ltac:(lia) _ H1).
+      destruct_hypos.
+    eexists. eexists.
+    repeat split.
+    + exact H.
+    + (* TODO *)
+Admitted.
+
+
+
+(* New LR *)
+Notation "Δ ',,' Γ '|-' e1 ≤ e2 ':' T" := (approx Δ Γ e1 e2 T)
+  ( at level 101
+  , e1 at level 0
+  , e2 at level 0
+  , T at level 0
+  , no associativity).
+
+
+Axiom approx_refl : ∀ (Δ : list (string * kind)) (Γ : list (string * ty)) (t : term) (T : ty),
+  Δ,, Γ |-+ t : T ->
+  Δ ,, Γ |- t ≤ t : T.
+
+Lemma approx_Let_NonRec_nil Δ Γ t T :
+  Δ ,, Γ |-+ (Let NonRec [] t) : T ->
+  Δ ,, Γ |- (Let NonRec [] t) ≤ t : T.
+Proof.
+  intros H_ty.
+  unfold approx.
+  assert (H_ty' : Δ ,, Γ |-+ t : T) by auto using has_type__Let_Nil_inv.
+  repeat split.
+  - assumption.
+  - assumption.
+  - intros k ρ γ γ' H_D H_G.
+    autorewrite with R.
+    intros j H_j_k r.
+    intros H_eval.
+    rewrite msubstA_LetNonRec_nil, msubst_LetNonRec_nil  in H_eval.
+    inversion_clear H_eval.
+    inversion_clear H.
+    assert (H_t_refl : Δ ,, Γ |- t ≤ t : T). { apply approx_refl. assumption. }
+    destruct H_t_refl as [ _ [ _ H_C]].
+    (* apply G_monotone with (Δ := Δ) (i := j) in H_G; try solve [assumption | lia]. *)
+    specialize (H_C k _ _ _ H_D H_G).
+    autorewrite with R in H_C.
+    specialize (H_C j1 ltac:(lia) _ H1).
+    destruct_hypos.
+    exists x, x0.
+    split.
+    + assumption.
+    + destruct H2.
+      * apply V_monotone with (Δ := Δ) (i := k - j) in H2;try solve [assumption | lia].
+        left. assumption.
+      * right. assumption.
+Qed.
